rocq-osiris/theories/lang/syntax.v
@@ -372,6 +372,9 @@ with sitem :=
   (* An [include] directive [include me]. *)
   | IInclude (me : mexpr)
 
+  (* An external declaration [external x = e]. *)
+  | IExternal (x : var) (e : expr)
+
   (* An extensible variant type extension [type t += cs]. *)
   | IExtend (cs : list name)
 
