rocq-osiris/theories/stdlib/proofs/array.v
@@ -2,7 +2,7 @@ From osiris.lang Require Import type_nel encode notations int.
 From osiris.program_logic Require Import program_logic.
 From osiris.proofmode Require Import proofmode.
 
-From osiris.stdlib Require Import translated_array.
+From osiris.stdlib Require Import og_array Externals.
 
 From iris Require Import ltac_tactics.
 
@@ -25,11 +25,14 @@ Section proof.
          imp m {{ λ a, ∃ (xs : list A), ⌜length xs = n⌝ ∗ ownArray a xs ∗
                                      [∗ list] i↦x ∈ xs, Φ i x }})%I.
 
-  Definition init := (EAnonFun __fun8).
+  Definition init := (EAnonFun __fun21).
 
   Lemma imp_init η :
+    lookup_name η "make" = ret Externals__array_make →
+    lookup_name η "unsafe_set" = ret Externals__array_set →
     ⊢ imp (eval η init) {{ λ c, □ iSpec τ[Z; val] c init_spec }}.
   Proof.
+    iIntros (Hlookup1 Hlookup2).
     iApply imp_EAnon_pers.
     iIntros "!> /=".
     iIntros (n f).
@@ -66,12 +69,14 @@ Section proof.
 
     iApply (imp_ELet_var (B:=array)).
     { (* Subgoal: [make l (f 0)] *)
-      iApply (imp_EArrayMake (A:=A) n). iPureIntro; assumption.
-      iApply imp_EPath; eauto.
-      { iApply (imp_EApp τ[Z]).
+      iApply (imp_EApp τ[Z;A]).
+      - iApply imp_EPath. { simpl; eassumption. } iApply array_make_spec.
+      - instantiate (1:=(λ n',⌜n'=n⌝)%I). iApply imp_EPath; auto.
+      - iApply (imp_EApp τ[Z]).
         iApply imp_EPath; auto.
         iApply imp_EInt.
-        iIntros (?) "-> %m H". iApply "H". iPureIntro; lia. } }
+        iIntros (?) "-> %m H". iApply "H". iPureIntro; lia.
+      - iIntros (?? ->) "HΦ %m Hm". iApply "Hm"; [ iPureIntro; assumption | iExact "HΦ" ]. }
     iIntros (res) "(%x & HΦx & #Harr & Hslice)".
 
     (* Subgoal: [for i = 1 to ... done; res]. *)
@@ -94,9 +99,15 @@ Section proof.
         iPoseProof (split_Slice 1 with "Hslice") as "[Hslice1 Hslice2]".
         reflexivity. done. iFrame. auto. }
 
-      iIntros "!>" (i' Hbound) "(Hslice1 & %xs & %Hlenxs & Hslice2 & HΦs)".
-      iApply (imp_EArraySet2 (A:=A)).
-      { instantiate (1:=(λ a', ⌜a'=res⌝)%I).
+      iIntros "!>" (i' Hbound) "(Hslice2 & %xs & %Hlenxs & Hslice1 & HΦs)".
+      rewrite (unroll_replicate x (n - i') 1); last lia. rewrite replicate_singleton.
+      iPoseProof (split_Slice with "Hslice2") as "[Hslice Hslice2]"; first reflexivity.
+      length. reflexivity.
+      iCombine ("Hslice1 Hslice") as "Hslice1".
+      iPoseProof (split_Slice with "Hslice1") as "Hslice1". reflexivity. lia.
+      iApply (imp_EApp τ[array;Z;A]).
+      { iApply imp_EPath. { simpl; eassumption. } iApply array_set_spec. }
+      { instantiate (1:=(λ a, ⌜a = res⌝)%I).
         iApply imp_EPath; auto. }
       { instantiate (1:=(λ i, ⌜i = i'⌝)%I).
         iApply imp_EPath; auto. }
@@ -104,35 +115,25 @@ Section proof.
         iApply imp_EPath; auto.
         instantiate (1:=(λ i, ⌜i = i'⌝)%I). iApply imp_EPath; auto.
         iIntros "% -> % H". iApply "H"; iPureIntro; lia. }
-
-      iIntros (?? y) "-> -> HΦ".
-      iFrame "#".
-      iCombine "Hslice2 Hslice1" as "Hslice".
-      iPoseProof (split_Slice with "Hslice") as "Hslice".
-      reflexivity. lia.
-
-      iFrame.
-      iSplit; iNext.
-      - iPureIntro. rewrite length_app length_replicate.
-        lia.
-      - iIntros "Hslice".
-        iPoseProof (split_Slice (i'+1) _ _ _ _ (xs ++ singleton y) (replicate (n - i' - 1) x)
-                     with "Hslice") as "[Hslice0 Hslicei]".
-        { insert. rewrite app_assoc.
-          f_equal. f_equal. lia. }
-        { length. lia. }
+      { iIntros (y?) "-> %a -> HΦ %m Hm".
+        iSpecialize ("Hm" with "Harr Hslice1 HΦ [] []").
+        { iPureIntro; lia. }
+        { iPureIntro; length; lia. }
+        iApply (imp_mono_ret with "Hm").
+        iIntros "!>" (_) "(% & HΦ & Hslice1)".
+        insert.
         replace (n - (i' + 1)) with (n - i' - 1) by lia.
-        iFrame.
-        iSplit; first (iPureIntro; length; lia).
+        iFrame. length.
+        iSplit; first (iPureIntro; lia).
         take.
         rewrite big_sepL_snoc. iFrame.
         rewrite /length in Hlenxs. rewrite Hlenxs.
-        iApply "HΦ". }
+        iApply "HΦ". } }
 
     iIntros "(Hslempty & %xs & %Hlen & Hslice & HΦs)".
     iApply imp_EPath; first auto.
-    take.
-    iFrame. length. rewrite Hlen.
+    unfold ownArray. length. take.
+    iFrame. rewrite Hlen.
     replace (n - 1 + 1) with n by lia.
     assert (n `max` 1 = n) as -> by lia.
     by iFrame "#".
